Chord serializers

examples/Chord.v
@@ -1,6 +1,14 @@
 Require Import String.
 Require Import Bvector.
 
+Require Import Cheerios.Core.
+Require Import Cheerios.Combinators.
+Require Import Cheerios.DeserializerMonad.
+Require Import Cheerios.Tactics.
+Require Import Cheerios.Types.
+
+Import DeserializerNotations.
+
 Section Chord.
 
 Parameter N : nat.
@@ -10,8 +18,35 @@ Definition bit_len := 8 * N.
 Definition id := Bvector.Bvector bit_len.
 Definition addr := String.string.
 
+(* pointer *)
 Record pointer := mkPointer { ptrId : id; ptrAddr : addr }.
 
+
+Definition pointer_serialize (ptr : pointer) : IOStreamWriter.t :=
+  serialize (ptrId ptr) +$+ serialize (ptrAddr ptr).
+
+Definition pointer_deserialize : ByteListReader.t pointer :=
+  id <- deserialize;;
+     addr <- deserialize;;
+     ByteListReader.ret (mkPointer id addr).
+
+Lemma pointer_serialize_deserialize_id : serialize_deserialize_id_spec pointer_serialize
+                                                                       pointer_deserialize.
+Proof.
+  intros.
+  unfold pointer_serialize, pointer_deserialize.
+  destruct a.
+  cheerios_crush.
+Qed.
+
+Instance pointer_Serializer : Serializer pointer.
+Proof.
+  exact {| serialize := pointer_serialize;
+             deserialize := pointer_deserialize;
+             serialize_deserialize_id := pointer_serialize_deserialize_id |}.
+Qed.
+
+(* payload *)
 Inductive payload :=
 | Busy : payload
 | GetBestPredecessor : pointer -> payload
@@ -24,12 +59,101 @@ Inductive payload :=
 | Ping : payload
 | Pong : payload.
 
+Definition payload_serialize (pl : payload) :=
+  match pl with
+  | Busy => serialize x00
+  | GetBestPredecessor ptr => serialize x01 +$+ serialize ptr
+  | GotBestPredecessor ptr => serialize x02 +$+ serialize ptr
+  | GetSuccList => serialize x03
+  | GotSuccList l => serialize x04 +$+ serialize l
+  | GetPredAndSuccs => serialize x05
+  | GotPredAndSuccs ptr l => serialize x06 +$+ serialize ptr +$+ serialize l
+  | Notify => serialize x07
+  | Ping => serialize x08
+  | Pong => serialize x09
+  end.
+
+Definition payload_deserialize :=
+  tag <- deserialize;;
+      match tag with
+      | x00 => ByteListReader.ret Busy
+      | x01 => ptr <- deserialize;;
+                   ByteListReader.ret (GetBestPredecessor ptr)
+      | x02 => ptr <- deserialize;;
+                   ByteListReader.ret (GotBestPredecessor ptr)
+      | x03 => ByteListReader.ret GetSuccList
+      | x04 => l <- deserialize;;
+                 ByteListReader.ret (GotSuccList l)
+      | x05 => ByteListReader.ret GetPredAndSuccs
+      | x06 => ptr <- deserialize;;
+                   l <- deserialize;;
+                   ByteListReader.ret (GotPredAndSuccs ptr l)
+      | x07 => ByteListReader.ret Notify
+      | x08 => ByteListReader.ret Ping
+      | x09 => ByteListReader.ret Pong
+      | _ => ByteListReader.error
+      end.
+
+Lemma payload_serialize_deserialize_id : serialize_deserialize_id_spec payload_serialize
+                                                                       payload_deserialize.
+Proof.
+  intros.
+  unfold payload_serialize, payload_deserialize.
+  destruct a;
+    repeat (cheerios_crush; simpl).
+Qed.
+
+Instance payload_Serializer : Serializer payload.
+Proof.
+  exact {| serialize := payload_serialize;
+             deserialize := payload_deserialize;
+             serialize_deserialize_id := payload_serialize_deserialize_id |}.
+Qed.
+
+(* timeout *)
 Inductive timeout :=
 | Tick : timeout
 | RectifyTick : timeout
 | KeepaliveTick : timeout
 | Request : addr -> payload -> timeout.
 
+Definition timeout_serialize (t : timeout) :=
+  match t with
+  | Tick => serialize x00
+  | RectifyTick => serialize x01
+  | KeepaliveTick => serialize x02
+  | Request a pl => serialize x03 +$+ serialize a +$+ serialize pl
+  end.
+
+Definition timeout_deserialize :=
+  tag <- deserialize;;
+      match tag with
+      | x00 => ByteListReader.ret Tick
+      | x01 => ByteListReader.ret RectifyTick
+      | x02 => ByteListReader.ret KeepaliveTick
+      | x03 => a <- deserialize;;
+                 pl <- deserialize;;
+                 ByteListReader.ret (Request a pl)
+      | _ => ByteListReader.error
+      end.
+
+Lemma timeout_serialize_deserialize_id : serialize_deserialize_id_spec timeout_serialize
+                                                                       timeout_deserialize.
+Proof.
+  intros.
+  unfold timeout_serialize, timeout_deserialize.
+  destruct a;
+    repeat (cheerios_crush; simpl).
+Qed.
+
+Instance timeout_Serializer : Serializer timeout.
+Proof.
+  exact {| serialize := timeout_serialize;
+             deserialize := timeout_deserialize;
+             serialize_deserialize_id := timeout_serialize_deserialize_id |}.
+Qed.
+
+(* query *)
 Inductive query :=
 | Rectify : pointer -> query
 | Stabilize : query
@@ -37,4 +161,43 @@ Inductive query :=
 | Join : pointer -> query
 | Join2 : pointer -> query.
 
+Definition query_serialize (q : query) :=
+  match q with
+  | Rectify ptr => serialize x00 +$+ serialize ptr
+  | Stabilize => serialize x01
+  | Stabilize2 ptr => serialize x02 +$+ serialize ptr
+  | Join ptr => serialize x03 +$+ serialize ptr
+  | Join2 ptr => serialize x04 +$+ serialize ptr
+  end.
+
+Definition query_deserialize :=
+  tag <- deserialize;;
+      match tag with
+      | x00 => ptr <- deserialize;;
+                   ByteListReader.ret (Rectify ptr)
+      | x01 => ByteListReader.ret Stabilize
+      | x02 => ptr <- deserialize;;
+                   ByteListReader.ret (Stabilize2 ptr)
+      | x03 => ptr <- deserialize;;
+                   ByteListReader.ret (Join ptr)
+      | x04 => ptr <- deserialize;;
+                   ByteListReader.ret (Join2 ptr)
+      | _ => ByteListReader.error
+      end.
+
+Lemma query_serialize_deserialize_id : serialize_deserialize_id_spec query_serialize
+                                                                       query_deserialize.
+Proof.
+  intros.
+  unfold query_serialize, query_deserialize.
+  destruct a;
+    repeat (cheerios_crush; simpl).
+Qed.
+
+Instance query_Serializer : Serializer query.
+Proof.
+  exact {| serialize := query_serialize;
+             deserialize := query_deserialize;
+             serialize_deserialize_id := query_serialize_deserialize_id |}.
+Qed.
 End Chord.
